coq_translation/examples-from-rust-book/error_handling/map_in_result_via_match.v
@@ -9,7 +9,7 @@ Definition ParseIntError := ParseIntError.t.
 Definition multiply
     (first_number_str : ref str)
     (second_number_str : ref str)
-    : Result :=
+    : Result i32 ParseIntError :=
   match first_number_str.["parse"] with
   | Ok (first_number) =>
     match second_number_str.["parse"] with
@@ -19,7 +19,7 @@ Definition multiply
   | Err (e) => Err e
   end.
 
-Definition print (result : Result) : unit :=
+Definition print (result : Result i32 ParseIntError) : unit :=
   match result with
   | Ok (n) =>
     _crate.io._print
